Sltu, Sltiu, and R0 in Inductive instead of special Register value

src/Machine.v
@@ -8,27 +8,32 @@ Require Import compiler.Riscv.
 Section Machine.
 
   Context {w: nat}.
-  Context {Register: Set}.
-  Context {Reg0: Register}.
-  Context {dec_Register: DecidableEq Register}.
+  Context {Reg: Set}.
+  Context {dec_Register: DecidableEq Reg}.
 
   Record RiscvMachine := mkRiscvMachine {
-    instructionMem: word w -> @Instruction Register;
-    registers: Register -> word w;
+    instructionMem: word w -> @Instruction Reg;
+    registers: Reg -> word w;
     pc: word w;
   }.
 
-  Instance IsRiscvMachine: @RiscvState w Register (State RiscvMachine) :=
+  Instance IsRiscvMachine: @RiscvState w Reg (State RiscvMachine) :=
   {|
-      R0 := Reg0;
-      getRegister := fun (reg: Register) =>
-        machine <- get;
-        Return (machine.(registers) reg);
-      setRegister := fun (reg: Register) (v: word w) =>
-        machine <- get;
-        match machine with
-        | mkRiscvMachine imem regs pc =>
-            put (mkRiscvMachine imem (fun reg2 => if dec (reg = reg2) then v else regs reg2) pc)
+      getRegister := fun (reg: (@Register Reg)) =>
+        match reg with
+        | RegO => Return $0
+        | RegS r => machine <- get; Return (machine.(registers) r)
+        end;
+      setRegister := fun (reg: (@Register Reg)) (v: word w) =>
+        match reg with
+        | RegO => Return tt
+        | RegS r => machine <- get;
+                    match machine with
+                    | mkRiscvMachine imem regs pc =>
+                        put (mkRiscvMachine imem 
+                                            (fun reg2 => if dec (r = reg2) then v else regs reg2)
+                                            pc)
+                    end
         end;
       loadInst := fun (addr: word w) =>
         im <- gets instructionMem;
@@ -42,9 +47,9 @@ Section Machine.
         end;
   |}.
 
-  Definition initialRiscvMachine(imem: list (@Instruction Register)): RiscvMachine := {|
+  Definition initialRiscvMachine(imem: list (@Instruction Reg)): RiscvMachine := {|
     instructionMem := fun (i: word w) => nth (wordToNat i) imem InfiniteJal;
-    registers := fun (r: Register) => $0;
+    registers := fun (r: Reg) => $0;
     pc := $0
   |}.
 
@@ -57,18 +62,18 @@ Existing Instance IsRiscvMachine.
 Module MachineTest.
 
   Definition m1: @RiscvMachine 4 nat := {|
-    instructionMem := fun (w: word 4) => Add 3 3 3;
+    instructionMem := fun (w: word 4) => Nop;
     registers := fun (reg: nat) => $22;
     pc := $33
   |}.
 
-  Definition myInst := (@IsRiscvMachine 4 nat 0 _).
+  Definition myInst := (@IsRiscvMachine 4 nat _).
   Existing Instance myInst.
 
   Definition prog1: State (@RiscvMachine 4 nat) (word 4) :=
-    x <- getRegister 2;
-    setRegister 2 (x ^+ $3);;
-    getRegister 4.
+    x <- getRegister (RegS 2);
+    setRegister (RegS 2) (x ^+ $3);;
+    getRegister (RegS 4).
 
   Goal evalState prog1 m1 = $6. reflexivity. Qed.
 
